Engine: fix everything for the new leaf definition

Engine/PikeTreeSeen.v
@@ -34,7 +34,7 @@ Axiom initial_nothing:
 
 (* The semantic states of the PikeTree algorithm *)
 Inductive pike_tree_seen_state : Type :=
-| PTSS (idx:nat) (active: list (tree * group_map)) (best: option leaf) (blocked: list (tree * group_map)) (seen:seentrees)
+| PTSS (inp:input) (active: list (tree * group_map)) (best: option leaf) (blocked: list (tree * group_map)) (seen:seentrees)
 | PTSS_final (best: option leaf).
 
 
@@ -43,39 +43,39 @@ Inductive pike_tree_seen_step : pike_tree_seen_state -> pike_tree_seen_state -> 
 | ptss_skip:
 (* skip an active tree if it has been seen before *)
 (* this is non-deterministic, we can also not skip it by using the other rules *)
-  forall idx t gm active best blocked seen
+  forall inp t gm active best blocked seen
     (SEEN: inseen seen t = true),
-    pike_tree_seen_step (PTSS idx ((t,gm)::active) best blocked seen) (PTSS idx active best blocked seen)
+    pike_tree_seen_step (PTSS inp ((t,gm)::active) best blocked seen) (PTSS inp active best blocked seen)
 | ptss_final:
 (* moving to a final state when there are no more active or blocked trees *)
-  forall idx best seen,
-    pike_tree_seen_step (PTSS idx [] best [] seen) (PTSS_final best)
+  forall inp best seen,
+    pike_tree_seen_step (PTSS inp [] best [] seen) (PTSS_final best)
 | ptss_nextchar:
   (* when the list of active trees is empty, restart from the blocked ones, proceeding to the next character *)
   (* resetting the seen trees *)
-  forall idx best blocked tgm seen,
-    pike_tree_seen_step (PTSS idx [] best (tgm::blocked) seen) (PTSS (idx + 1) (tgm::blocked) best [] initial_seentrees)
+  forall inp best blocked tgm seen,
+    pike_tree_seen_step (PTSS inp [] best (tgm::blocked) seen) (PTSS (next_inp inp) (tgm::blocked) best [] initial_seentrees)
 | ptss_active:
   (* generated new active trees: add them in front of the low-priority ones *)
-  forall idx t gm active best blocked nextactive seen1 seen2
-    (STEP: tree_bfs_step t gm idx = StepActive nextactive)
+  forall inp t gm active best blocked nextactive seen1 seen2
+    (STEP: tree_bfs_step t gm (idx inp) = StepActive nextactive)
     (ADD_SEEN: add_seentrees seen1 t = seen2),
-    pike_tree_seen_step (PTSS idx ((t,gm)::active) best blocked seen1) (PTSS idx (nextactive++active) best blocked seen2)
+    pike_tree_seen_step (PTSS inp ((t,gm)::active) best blocked seen1) (PTSS inp (nextactive++active) best blocked seen2)
 | ptss_match:
   (* a match is found, discard remaining low-priority active trees *)
-  forall idx t gm active best blocked seen1 seen2
-    (STEP: tree_bfs_step t gm idx = StepMatch)
+  forall inp t gm active best blocked seen1 seen2
+    (STEP: tree_bfs_step t gm (idx inp) = StepMatch)
     (ADD_SEEN: add_seentrees seen1 t = seen2),
-    pike_tree_seen_step (PTSS idx ((t,gm)::active) best blocked seen1) (PTSS idx [] (Some gm) blocked seen2)
+    pike_tree_seen_step (PTSS inp ((t,gm)::active) best blocked seen1) (PTSS inp [] (Some (inp,gm)) blocked seen2)
 | ptss_blocked:
 (* add the new blocked thread after the previous ones *)
-  forall idx t gm active best blocked newt seen1 seen2
-    (STEP: tree_bfs_step t gm idx = StepBlocked newt)
+  forall inp t gm active best blocked newt seen1 seen2
+    (STEP: tree_bfs_step t gm (idx inp) = StepBlocked newt)
     (ADD_SEEN: add_seentrees seen1 t = seen2),
-    pike_tree_seen_step (PTSS idx ((t,gm)::active) best blocked seen1) (PTSS idx active best (blocked ++ [(newt,gm)]) seen2).
+    pike_tree_seen_step (PTSS inp ((t,gm)::active) best blocked seen1) (PTSS inp active best (blocked ++ [(newt,gm)]) seen2).
 
-Definition pike_tree_seen_initial_state (t:tree) : pike_tree_seen_state :=
-  (PTSS 0 [(t, GroupMap.empty)] None [] initial_seentrees).
+Definition pike_tree_seen_initial_state (t:tree) (i:input) : pike_tree_seen_state :=
+  (PTSS i [(t, GroupMap.empty)] None [] initial_seentrees).
 
 
 (** * Pike Tree Seen Correction  *)
@@ -83,32 +83,32 @@ Definition pike_tree_seen_initial_state (t:tree) : pike_tree_seen_state :=
 
 (** * Non-deterministic tree results *)
 (* any possible result after skipping or not any sub-tree in the seen set *)
-Inductive tree_nd: tree -> group_map -> nat -> seentrees -> option leaf -> Prop :=
+Inductive tree_nd: tree -> group_map -> input -> seentrees -> option leaf -> Prop :=
 | tr_skip:
-  forall seen t gm idx
+  forall seen t gm inp
     (SEEN: inseen seen t = true),
-    tree_nd t gm idx seen None
+    tree_nd t gm inp seen None
 | tr_mismatch:
-  forall gm idx seen, tree_nd Mismatch gm idx seen None
+  forall gm inp seen, tree_nd Mismatch gm inp seen None
 | tr_match:
-  forall gm idx seen, tree_nd Match gm idx seen (Some gm)
+  forall gm inp seen, tree_nd Match gm inp seen (Some (inp,gm))
 | tr_choice:
-  forall t1 t2 gm idx l1 l2 seen
-    (TR1: tree_nd t1 gm idx seen l1)
-    (TR2: tree_nd t2 gm idx seen l2),
-    tree_nd (Choice t1 t2) gm idx seen (seqop l1 l2)
+  forall t1 t2 gm inp l1 l2 seen
+    (TR1: tree_nd t1 gm inp seen l1)
+    (TR2: tree_nd t2 gm inp seen l2),
+    tree_nd (Choice t1 t2) gm inp seen (seqop l1 l2)
 | tr_read:
-  forall t cd gm idx l seen
-    (TR: tree_nd t gm (idx+1) seen l),
-    tree_nd (Read cd t) gm idx seen l
+  forall t cd gm inp l seen
+    (TR: tree_nd t gm (next_inp inp) seen l),
+    tree_nd (Read cd t) gm inp seen l
 | tr_progress:
-  forall t gm idx l seen
-    (TR: tree_nd t gm idx seen l),
-    tree_nd (Progress t) gm idx seen l
+  forall t gm inp l seen
+    (TR: tree_nd t gm inp seen l),
+    tree_nd (Progress t) gm inp seen l
 | tr_groupaction:
-  forall t act gm idx l seen
-    (TR: tree_nd t (GroupMap.update idx act gm) idx seen l),
-    tree_nd (GroupAction act t) gm idx seen l.
+  forall t act gm inp l seen
+    (TR: tree_nd t (GroupMap.update (idx inp) act gm) inp seen l),
+    tree_nd (GroupAction act t) gm inp seen l.
 (* To keep this relation as simple as possible, it does not compute
 the results of a tree which does not corespond to the regexes
 supported by the engine. We could support them, but we won't need them
@@ -118,21 +118,21 @@ and it would require adding a direction as argument *)
 
 (* the normal result, obtained with function tree_res without skipping anything, is a possible result *)
 Lemma tree_res_nd:
-  forall t gm idx seen,
+  forall t gm inp seen,
     pike_subtree t -> 
-    tree_nd t gm idx seen (tree_res t gm idx forward).
+    tree_nd t gm inp seen (tree_res t gm inp forward).
 Proof.
   intros t. induction t; intros; simpl; try solve[inversion H]; try solve[pike_subset; constructor; auto].
 Qed.
 
 (* when there is nothing in seen, there is only one possible result *)
 Lemma tree_nd_initial:
-  forall t gm idx res,
+  forall t gm inp res,
     pike_subtree t ->
-    tree_nd t gm idx initial_seentrees res ->
-    res = tree_res t gm idx forward.
+    tree_nd t gm inp initial_seentrees res ->
+    res = tree_res t gm inp forward.
 Proof.
-  intros t gm idx res PIKE H.
+  intros t gm inp res PIKE H.
   remember initial_seentrees as init.
   induction H; simpl; pike_subset; auto.
   - subst. rewrite initial_nothing in SEEN. inversion SEEN.
@@ -140,21 +140,21 @@ Proof.
     specialize (IHtree_nd2 H4 (@eq_refl _ _)). subst. auto.
 Qed.
 
-Inductive list_nd: list (tree * group_map) -> nat -> seentrees -> option leaf -> Prop :=
+Inductive list_nd: list (tree * group_map) -> input -> seentrees -> option leaf -> Prop :=
 | tlr_nil:
-  forall idx seen, list_nd [] idx seen None
+  forall inp seen, list_nd [] inp seen None
 | tlr_cons:
-  forall t gm active idx seen l1 l2 l3
-    (TR: tree_nd t gm idx seen l1)
-    (TLR: list_nd active idx seen l2)
+  forall t gm active inp seen l1 l2 l3
+    (TR: tree_nd t gm inp seen l1)
+    (TLR: list_nd active inp seen l2)
     (SEQ: l3 = seqop l1 l2),
-    list_nd ((t,gm)::active) idx seen l3.
+    list_nd ((t,gm)::active) inp seen l3.
 
 (* the normal result for a list, without skipping anything, is a possible result *)
 Lemma list_result_nd:
-  forall active idx seen,
+  forall active inp seen,
     pike_list active -> 
-    list_nd active idx seen (list_result active idx).
+    list_nd active inp seen (list_result active inp).
 Proof.
   intros active. induction active; try destruct a as [t gm]; intros; pike_subset; try constructor.
   rewrite list_result_cons.
@@ -163,12 +163,12 @@ Qed.
 
 (* when there is nothing in seen, there is only one possible result *)
 Lemma list_nd_initial:
-  forall l idx res,
+  forall l inp res,
     pike_list l ->
-    list_nd l idx initial_seentrees res ->
-    res = list_result l idx.
+    list_nd l inp initial_seentrees res ->
+    res = list_result l inp.
 Proof.
-  intros l idx res PIKE H.
+  intros l inp res PIKE H.
   remember initial_seentrees as init.
   induction H; simpl; auto; pike_subset.
   rewrite list_result_cons. specialize (IHlist_nd H1 (eq_refl _)). subst.
@@ -176,24 +176,24 @@ Proof.
 Qed.
 
 
-Inductive state_nd: nat -> list (tree*group_map) -> option leaf -> list (tree*group_map) -> seentrees -> option leaf -> Prop :=
+Inductive state_nd: input -> list (tree*group_map) -> option leaf -> list (tree*group_map) -> seentrees -> option leaf -> Prop :=
 | sr:
-  forall blocked active best idx seen r1 r2 rseq
-    (BLOCKED: list_result blocked (idx+1) = r1)
-    (ACTIVE: list_nd active idx seen r2)
+  forall blocked active best inp seen r1 r2 rseq
+    (BLOCKED: list_result blocked (next_inp inp) = r1)
+    (ACTIVE: list_nd active inp seen r2)
     (SEQ: rseq = seqop r1 (seqop r2 best)),
-    state_nd idx active best blocked seen rseq.
+    state_nd inp active best blocked seen rseq.
 
 (* Invariant of the PikeTreeSeen execution *)
 (* at any moment, all the possible results of the current state are all equal (equal to the first result of the original tree) *)
 (* at any moment, all trees manipulated by the algorithms are trees for the subset of regexes supported  *)
 Inductive piketreeinv: pike_tree_seen_state -> option leaf -> Prop :=
 | pi:
-  forall result blocked active best idx seen
-    (SAMERES: forall res, state_nd idx active best blocked seen res -> res = result)
+  forall result blocked active best inp seen
+    (SAMERES: forall res, state_nd inp active best blocked seen res -> res = result)
     (SUBSET_AC: pike_list active)
     (SUBSET_BL: pike_list blocked),
-    piketreeinv (PTSS idx active best blocked seen) result
+    piketreeinv (PTSS inp active best blocked seen) result
 | sr_final:
   forall best,
     piketreeinv (PTSS_final best) best.
@@ -201,9 +201,9 @@ Inductive piketreeinv: pike_tree_seen_state -> option leaf -> Prop :=
 (** * Initialization  *)
 
 Lemma init_piketree_inv:
-  forall t,
+  forall t inp,
     pike_subtree t -> 
-    piketreeinv (pike_tree_seen_initial_state t) (tree_res t GroupMap.empty 0 forward).
+    piketreeinv (pike_tree_seen_initial_state t inp) (tree_res t GroupMap.empty inp forward).
 Proof.
   intros t. unfold pike_tree_seen_initial_state. constructor; pike_subset; auto.
   intros res STATEND. inversion STATEND; subst.
@@ -214,23 +214,23 @@ Qed.
 
 (** * Non deterministic results lemmas  *)
 
-(* a tree having no results is independent of the gm and the idx *)
+(* a tree having no results is independent of the gm and the inp *)
 Lemma no_tree_result:
-  forall t gm1 gm2 idx1 idx2
-    (NORES: tree_res t gm1 idx1 forward = None),
-    tree_res t gm2 idx2 forward = None.
+  forall t gm1 gm2 inp1 inp2
+    (NORES: tree_res t gm1 inp1 forward = None),
+    tree_res t gm2 inp2 forward = None.
 Proof.
   intros. rewrite first_tree_leaf. rewrite first_tree_leaf in NORES.
-  destruct (tree_leaves t gm1 idx1 forward) eqn:HTL.
+  destruct (tree_leaves t gm1 inp1 forward) eqn:HTL.
   2: { inversion NORES. }
   eapply leaves_group_map_indep in HTL. rewrite HTL. auto.
 Qed.    
 
 (* the same is true for a non-deterministic result *)
 Lemma no_tree_result_nd:
-  forall t seen gm1 gm2 idx1 idx2
-    (NORES: tree_nd t gm1 idx1 seen None),
-    tree_nd t gm2 idx2 seen None.
+  forall t seen gm1 gm2 inp1 inp2
+    (NORES: tree_nd t gm1 inp1 seen None),
+    tree_nd t gm2 inp2 seen None.
 Proof.
   intros t. induction t; intros;
     try solve[inversion NORES; subst; try solve[constructor; auto]; try solve [constructor; eapply IHt; eauto]].
@@ -244,13 +244,13 @@ Qed.
 
 (* skipping over a new tree doesn't change the result if the tree that is being skipped does not have results *)
 Lemma add_seen:
-  forall t seen tseen gm idx res
-    (NORES: tree_res tseen gm idx forward = None)
-    (TREEND: tree_nd t gm idx (add_seentrees seen tseen) res)
+  forall t seen tseen gm inp res
+    (NORES: tree_res tseen gm inp forward = None)
+    (TREEND: tree_nd t gm inp (add_seentrees seen tseen) res)
     (SUBSET: pike_subtree tseen),
-    tree_nd t gm idx seen res.
+    tree_nd t gm inp seen res.
 Proof.
-  intros t seen tseen gm idx res NORES TREEND SUBSET.
+  intros t seen tseen gm inp res NORES TREEND SUBSET.
   remember (add_seentrees seen tseen) as add.
   induction TREEND; subst; try solve[constructor; auto];
     try solve [constructor; apply IHTREEND; auto; eapply no_tree_result; eauto].
@@ -261,13 +261,13 @@ Qed.
 
 (* same lemma generalizes to lists of trees *)
 Lemma list_add_seen:
-  forall l seen tseen gm idx res
-    (NORES: tree_res tseen gm idx forward = None)
-    (LISTND: list_nd l idx (add_seentrees seen tseen) res)
+  forall l seen tseen gm inp res
+    (NORES: tree_res tseen gm inp forward = None)
+    (LISTND: list_nd l inp (add_seentrees seen tseen) res)
     (SUBSET: pike_subtree tseen),
-    list_nd l idx seen res.
+    list_nd l inp seen res.
 Proof.
-  intros l seen tseen gm idx res NORES LISTND SUBSET.
+  intros l seen tseen gm inp res NORES LISTND SUBSET.
   remember (add_seentrees seen tseen) as add.
   induction LISTND; subst; econstructor; eauto.
   eapply add_seen; eauto. eapply no_tree_result; eauto.
@@ -275,12 +275,12 @@ Qed.
 
 (* skipping over a new tree doesn't change the result if the tree that is being skipped can produce a None result *)
 Lemma add_seen_nd:
-  forall t seen tseen gm idx res
-    (NORES: tree_nd tseen gm idx seen None)
-    (TREEND: tree_nd t gm idx (add_seentrees seen tseen) res),
-    tree_nd t gm idx seen res.
+  forall t seen tseen gm inp res
+    (NORES: tree_nd tseen gm inp seen None)
+    (TREEND: tree_nd t gm inp (add_seentrees seen tseen) res),
+    tree_nd t gm inp seen res.
 Proof.
-  intros t seen tseen gm idx res NORES TREEND.
+  intros t seen tseen gm inp res NORES TREEND.
   remember (add_seentrees seen tseen) as add.
   induction TREEND; subst; try solve[constructor; auto];
     try solve [constructor; apply IHTREEND; auto; eapply no_tree_result_nd; eauto].
@@ -291,12 +291,12 @@ Qed.
 
 (* same lemma generalizes to lists of trees *)
 Lemma list_add_seen_nd:
-  forall l seen tseen gm idx res
-    (NORES: tree_nd tseen gm idx seen None)
-    (LISTND: list_nd l idx (add_seentrees seen tseen) res),
-    list_nd l idx seen res.
+  forall l seen tseen gm inp res
+    (NORES: tree_nd tseen gm inp seen None)
+    (LISTND: list_nd l inp (add_seentrees seen tseen) res),
+    list_nd l inp seen res.
 Proof.
-  intros l seen tseen gm idx res NORES LISTND.
+  intros l seen tseen gm inp res NORES LISTND.
   remember (add_seentrees seen tseen) as add.
   induction LISTND; subst; econstructor; eauto.
   eapply add_seen_nd; eauto. eapply no_tree_result_nd; eauto.
@@ -316,12 +316,12 @@ Fixpoint size (t:tree) : nat :=
 (* skipping over a new tree does not change the result of another tree if we know that the newly *)
 (* skipped over tree cannot appear in the tree we compute the result of *)
 Lemma add_parent_tree:
-  forall tseen t res seen gm idx
+  forall tseen t res seen gm inp
     (SIZE: size t < size tseen)
-    (TREEND: tree_nd t gm idx (add_seentrees seen tseen) res),
-    tree_nd t gm idx seen res.
+    (TREEND: tree_nd t gm inp (add_seentrees seen tseen) res),
+    tree_nd t gm inp seen res.
 Proof.
-  intros tseen t res seen gm idx SIZE TREEND.
+  intros tseen t res seen gm inp SIZE TREEND.
   remember (add_seentrees seen tseen) as add.
   induction TREEND; subst; simpl in SIZE;
     try solve [constructor; apply IHTREEND; auto; lia].
@@ -359,7 +359,7 @@ Proof.
   - constructor; pike_subset; auto. intros res STATEND. inversion STATEND; subst.
     apply list_nd_initial in ACTIVE.
     2: { destruct tgm. pike_subset; auto. }
-    simpl. subst. specialize (SAMERES (seqop (list_result (tgm::blocked0) (idx+1)) (seqop None best))).
+    simpl. subst. specialize (SAMERES (seqop (list_result (tgm::blocked0) (next_inp inp)) (seqop None best))).
     simpl in SAMERES. apply SAMERES. econstructor; constructor.
   (* mismatch *)
   - simpl. constructor; pike_subset; auto. intros res STATEND. inversion STATEND; subst. apply SAMERES.
@@ -375,7 +375,7 @@ Proof.
     2: { simpl. lia. }
     apply add_parent_tree in TR0.
     2: { simpl. lia. }
-    assert (PARENT: tree_nd (Choice t1 t2) gm idx seen (seqop l1 l0)).
+    assert (PARENT: tree_nd (Choice t1 t2) gm inp seen (seqop l1 l0)).
     { apply tr_choice; auto. }
     (* case analysis: did t contribute to the result? *)
     destruct (seqop l1 l0) as [leaf|] eqn:CHOICE.
@@ -397,7 +397,7 @@ Proof.
     apply SAMERES.
     apply add_parent_tree in TR.
     2: { simpl. lia. }
-    assert (PARENT: tree_nd (Progress t) gm idx seen l1).
+    assert (PARENT: tree_nd (Progress t) gm inp seen l1).
     { apply tr_progress; auto. }
     (* case analysis: did t contribute to the result? *)
     destruct l1 as [leaf1|].
@@ -416,7 +416,7 @@ Proof.
     apply SAMERES.
     apply add_parent_tree in TR.
     2: { simpl. lia. }
-    assert (PARENT: tree_nd (GroupAction g t) gm idx seen l1).
+    assert (PARENT: tree_nd (GroupAction g t) gm inp seen l1).
     { apply tr_groupaction; auto. }
     (* case analysis: did t contribute to the result? *)
     destruct l1 as [leaf1|].
@@ -435,8 +435,8 @@ Proof.
   - destruct t; inversion STEP; subst. constructor; pike_subset; auto.
     intros res STATEND. inversion STATEND; subst.
     inversion ACTIVE; subst. simpl. 
-    apply SAMERES. eapply sr with (r2:=Some gm); eauto.
-    replace (Some gm) with (seqop (Some gm) (list_result active0 idx)) by (simpl; auto).
+    apply SAMERES. eapply sr with (r2:=Some (inp,gm)); eauto.
+    replace (Some (inp,gm)) with (seqop (Some (inp,gm)) (list_result active0 inp)) by (simpl; auto).
     econstructor; auto.
     + apply tr_match.
     + apply list_result_nd; auto.
@@ -445,21 +445,21 @@ Proof.
     intros res STATEND. inversion STATEND; subst.
     apply SAMERES.
     rewrite list_result_app. rewrite list_result_cons.
-    replace (list_result [] (idx+1)) with (None:option leaf).
+    replace (list_result [] (next_inp inp)) with (None:option leaf).
     2: { unfold list_result, seqop_list. simpl. auto. }
     rewrite seqop_none. rewrite <- seqop_assoc. rewrite seqop_assoc with (o3:=best).
     econstructor; eauto.
-    destruct (tree_res newt gm (idx+1)) eqn:REST.
+    destruct (tree_res newt gm (next_inp inp)) eqn:REST.
     (* if the blocked tree contained a match, then we don't care about the result of active *)
     (* we can simply use the result obtained without skipping anything *)
     + eapply tlr_cons.
       * apply tree_res_nd. pike_subset.
       * apply list_result_nd; auto.
-      * simpl. rewrite REST. simpl. auto.
+      * simpl. unfold next_inp in REST. rewrite REST. simpl. auto.
     + eapply tlr_cons.
       (* if the blocked tree did not contain a match, we prove that the adding it to the seen set *)
       (* does not change the skipping of the following active trees, using list_add_seen *)
       * apply tree_res_nd. pike_subset.
       * eapply list_add_seen in ACTIVE; eauto. pike_subset.
-      * simpl. rewrite REST. simpl. auto.
+      * simpl. unfold next_inp in REST. rewrite REST. simpl. auto.
 Qed.
